WIP: separation logic stub

src/Locker.v
@@ -6,12 +6,14 @@ Require Import Arith.
 Require Import Omega.
 Require Bool.
 Require Import FoldIn.
+Require Storage.
+Require EqDec.
 
 Module Unbounded (S : Storage.Interface).
 
 Definition Offset := nat.
 
-Variable Key : Storage.Keq_dec.
+Variable Key : Keq_dec.
 Variable Value : Set.
 Variable TxPayload : Set.
 
@@ -19,8 +21,8 @@ Variable TxPayload : Set.
 Record Tx :=
   mkTx
     { last_imported_offset : Offset;
-      reads : list (Storage.KT Key * Offset);
-      writes : list (Storage.KT Key * Offset);
+      reads : list (KT Key * Offset);
+      writes : list (KT Key * Offset);
       commit : bool;
       payload : TxPayload;
     }.
@@ -39,7 +41,7 @@ Record State :=
       seqnos : Seqnos;
     }.
 
-Definition get_seqno (k : Storage.KT Key) (s : State) : Offset :=
+Definition get_seqno (k : KT Key) (s : State) : Offset :=
   match S.get k (seqnos s) with
   | Some v => v
   | None   => 0
@@ -97,7 +99,7 @@ Module L := Unbounded(S). Import L.
 Module SP := Storage.Properties(S). Import SP.
 Module SE := Storage.Equality(S). Import SE.
 
-Definition tx_keys (tx : Tx) : list (Storage.KT L.Key) :=
+Definition tx_keys (tx : Tx) : list (KT L.Key) :=
   match tx with
   | {| reads := rr; writes := ww |} =>
     map (fun x => match x with (x, _) => x end) (rr ++ ww)
@@ -130,9 +132,9 @@ Lemma subset_s_eq_forallb : forall ws o1 o2 s1 s2 l,
     let S2 := mkState ws o2 s2 in
     subset_s_eq l S1 S2 ->
     forallb
-      (fun x : Storage.KT L.Key * nat => let (k, v) := x in v =? get_seqno k S1) l =
+      (fun x : KT L.Key * nat => let (k, v) := x in v =? get_seqno k S1) l =
     forallb
-      (fun x : Storage.KT L.Key * nat => let (k, v) := x in v =? get_seqno k S2) l.
+      (fun x : KT L.Key * nat => let (k, v) := x in v =? get_seqno k S2) l.
 Proof.
   intros.
   repeat rewrite forallb_forallb'.
@@ -195,8 +197,7 @@ Lemma consume_tx_subset_eq_p : forall hwm S1 S2 tx,
 Proof.
   intros hwm S1 S2 tx Hws Hrl Hwl.
   unfold consume_tx.
-  specialize (check_tx_subset_eq_p hwm S1 S2 tx) as Hcheck.
-  rewrite Hcheck.
+  rewrite (check_tx_subset_eq_p hwm S1 S2 tx).
   destruct (check_tx S2 hwm tx);
     destruct S1 as [ws1 o1 s1];
     destruct S2 as [ws2 o2 s2];
@@ -204,125 +205,142 @@ Proof.
     simpl in *;
     rewrite Hws in *;
     split; split; try easy.
-  - unfold update_seqnos. simpl in *.
-  -
-  - split; try easy.
-    split.
-  - simpl.
-    destruct S1 as [ws ]
-
-
-
-Inductive ReachableState {window_size : nat} {offset : Offset} : State -> Prop :=
-| InitState :
-    ReachableState (mkState window_size offset S.new)
-| NextState : forall (tx : Tx) seqnos,
-    let s := mkState window_size offset seqnos in
-    ReachableState s ->
-    ReachableState (next_state s (S offset) tx).
-
-Definition s_eq (s1 s2 : State) :=
-  match s1, s2 with
-  | (mkState ws1 o1 s1), (mkState ws2 o2 s2) => ws1 = ws2 /\ o1 = o2 /\ s1 =s= s2
-  end.
-
-Notation "a =S= b" := (s_eq a b) (at level 50).
-
-Definition replay_erases_initial_stateP :=
-  forall (tlog : Tlog) (o0 : Offset),
-    let ws := List.length tlog in
-    forall s1 s2,
-      replay' o0 tlog (mkState ws o0 (collect_garbage ws o0 s1)) =S=
-      replay' o0 tlog (mkState ws o0 (collect_garbage ws o0 s2)).
-
-Definition garbage_collect_works :=
-  forall ws offset seqnos,
-    let s' := collect_garbage ws offset seqnos in
-    forallS s' (fun k Hin => match getT k s' Hin with
-                          | (_, v) => offset - v < ws
-                          end).
-
-Lemma replay_erases_initial_state :
-  garbage_collect_works -> replay_erases_initial_stateP.
-Proof.
-  unfold replay_erases_initial_stateP. intros Hgc tlog o s1 s2.
-  set (S1 := {| sync_window_size := length tlog; my_tlogn := o; seqnos := collect_garbage (length tlog) o s1 |}).
-  set (S2 := {| sync_window_size := length tlog; my_tlogn := o; seqnos := collect_garbage (length tlog) o s2 |}).
-  replace tlog with (rev (rev tlog)) by apply rev_involutive.
-  remember (rev tlog) as tlogr.
-  induction tlogr as [|tx tlogr IH].
-  { simpl.
-    repeat split; auto.
-    rewrite <-rev_length. rewrite <- Heqtlogr. simpl.
-    assert (Hempty : forall k s, S.get k (collect_garbage 0 o s) = None).
-    { intros.
-      unfold collect_garbage.
+  - subst.
+    unfold update_seqnos. simpl in *.
+    (* Here it's beneficial to iterate the list backwards to make a
+    goal closely matching with the inductive hypothesis: *)
+    replace wl with (rev (rev wl)) by apply rev_involutive.
+    induction (rev wl).
+    + simpl. assumption.
+    + simpl. repeat rewrite fold_left_app. simpl.
       admit.
-    }
-    intros k.
-    repeat rewrite Hempty. reflexivity.
-  }
-  { simpl.
+  - unfold update_seqnos. simpl in *.
+    (* Here it's beneficial to iterate the list backwards to make a
+    goal closely matching with the inductive hypothesis: *)
+    replace wl with (rev (rev wl)) by apply rev_involutive.
+    induction (rev wl).
+    + easy.
+    + simpl. repeat rewrite fold_left_app. simpl.
+Abort.
+End UnboundedSpec.
 
-    set (l := length tlog) in *.
-    replace (length (tx :: tlog)) with (S l) in * by reflexivity.
-    set (s1' := collect_garbage l o s1) in *.
-    set (s2' := collect_garbage l o s2) in *.
-    set (s1'' := collect_garbage (S l) o s1) in *.
-    set (s2'' := collect_garbage (S l) o s2) in *.
-    simpl.
-    destruct tx.
-    - (* Write transaction *)
-      destruct (o - local_tlogn w <? S l) in *.
-      + give_up.
-      +
-  }
-
-    specialize (Hgc 0 o s1) as Hs1.
-    specialize (Hgc 0 o s2) as Hs2.
-    simpl in *.
-    remember (S.get k s1) as v1.
-    remember (S.get k s2) as v2.
-    destruct v1; destruct v2.
-
-    specialize (Hgc 0 o s1) as Hs1.
-    specialize (Hgc 0 o s2) as Hs2.
-
-
-    unfold garbage_collect_works in Hgc.
-
-    destruct Hs1; destruct Hs2; simpl; auto; destruct tx as [txw].
-    - unfold next_state.v
-      cbv.
-      remember (S o0 - (local_tlogn txw) <? 0) as ss.
-      destruct (S o0 - (local_tlogn txw) <? 0).
-      +
+(*   - split; try easy. *)
+(*     split. *)
+(*   - simpl. *)
+(*     destruct S1 as [ws ] *)
 
 
 
+(* Inductive ReachableState {window_size : nat} {offset : Offset} : State -> Prop := *)
+(* | InitState : *)
+(*     ReachableState (mkState window_size offset S.new) *)
+(* | NextState : forall (tx : Tx) seqnos, *)
+(*     let s := mkState window_size offset seqnos in *)
+(*     ReachableState s -> *)
+(*     ReachableState (next_state s (S offset) tx). *)
+
+(* Definition s_eq (s1 s2 : State) := *)
+(*   match s1, s2 with *)
+(*   | (mkState ws1 o1 s1), (mkState ws2 o2 s2) => ws1 = ws2 /\ o1 = o2 /\ s1 =s= s2 *)
+(*   end. *)
+
+(* Notation "a =S= b" := (s_eq a b) (at level 50). *)
+
+(* Definition replay_erases_initial_stateP := *)
+(*   forall (tlog : Tlog) (o0 : Offset), *)
+(*     let ws := List.length tlog in *)
+(*     forall s1 s2, *)
+(*       replay' o0 tlog (mkState ws o0 (collect_garbage ws o0 s1)) =S= *)
+(*       replay' o0 tlog (mkState ws o0 (collect_garbage ws o0 s2)). *)
+
+(* Definition garbage_collect_works := *)
+(*   forall ws offset seqnos, *)
+(*     let s' := collect_garbage ws offset seqnos in *)
+(*     forallS s' (fun k Hin => match getT k s' Hin with *)
+(*                           | (_, v) => offset - v < ws *)
+(*                           end). *)
+
+(* Lemma replay_erases_initial_state : *)
+(*   garbage_collect_works -> replay_erases_initial_stateP. *)
+(* Proof. *)
+(*   unfold replay_erases_initial_stateP. intros Hgc tlog o s1 s2. *)
+(*   set (S1 := {| sync_window_size := length tlog; my_tlogn := o; seqnos := collect_garbage (length tlog) o s1 |}). *)
+(*   set (S2 := {| sync_window_size := length tlog; my_tlogn := o; seqnos := collect_garbage (length tlog) o s2 |}). *)
+(*   replace tlog with (rev (rev tlog)) by apply rev_involutive. *)
+(*   remember (rev tlog) as tlogr. *)
+(*   induction tlogr as [|tx tlogr IH]. *)
+(*   { simpl. *)
+(*     repeat split; auto. *)
+(*     rewrite <-rev_length. rewrite <- Heqtlogr. simpl. *)
+(*     assert (Hempty : forall k s, S.get k (collect_garbage 0 o s) = None). *)
+(*     { intros. *)
+(*       unfold collect_garbage. *)
+(*       admit. *)
+(*     } *)
+(*     intros k. *)
+(*     repeat rewrite Hempty. reflexivity. *)
+(*   } *)
+(*   { simpl. *)
+
+(*     set (l := length tlog) in *. *)
+(*     replace (length (tx :: tlog)) with (S l) in * by reflexivity. *)
+(*     set (s1' := collect_garbage l o s1) in *. *)
+(*     set (s2' := collect_garbage l o s2) in *. *)
+(*     set (s1'' := collect_garbage (S l) o s1) in *. *)
+(*     set (s2'' := collect_garbage (S l) o s2) in *. *)
+(*     simpl. *)
+(*     destruct tx. *)
+(*     - (* Write transaction *) *)
+(*       destruct (o - local_tlogn w <? S l) in *. *)
+(*       + give_up. *)
+(*       + *)
+(*   } *)
+
+(*     specialize (Hgc 0 o s1) as Hs1. *)
+(*     specialize (Hgc 0 o s2) as Hs2. *)
+(*     simpl in *. *)
+(*     remember (S.get k s1) as v1. *)
+(*     remember (S.get k s2) as v2. *)
+(*     destruct v1; destruct v2. *)
+
+(*     specialize (Hgc 0 o s1) as Hs1. *)
+(*     specialize (Hgc 0 o s2) as Hs2. *)
+
+
+(*     unfold garbage_collect_works in Hgc. *)
+
+(*     destruct Hs1; destruct Hs2; simpl; auto; destruct tx as [txw]. *)
+(*     - unfold next_state.v *)
+(*       cbv. *)
+(*       remember (S o0 - (local_tlogn txw) <? 0) as ss. *)
+(*       destruct (S o0 - (local_tlogn txw) <? 0). *)
+(*       + *)
 
 
 
-Theorem replay_state_is_consistent :
-  forall (* ..for all window size 'ws' and transaction log 'tlog'
-       containing 'high_wm_offset' entries... *)
-    (ws : nat)
-    (tlog : Tlog)
-    (* ...any two followers starting from a valid offset... *)
-    start_offset1 (Hso1 : start_offset1 <= length tlog)
-    start_offset2 (Hso2 : start_offset2 <= length tlog)
-  , (* ...will eventually reach the same state: *)
-    replay tlog (initial_state ws start_offset1) =
-    replay tlog (initial_state ws start_offset2).
-Proof.
-  intros.
-  unfold initial_state.
-  remember (rev tlog) as tlog'.
-  induction rtlog;
-    rewrite <- rev_length in *.
-  - (* Tlog is empty *)
-    simpl in *. destruct Heqrtlog.
-    apply le_n_0_eq in Hso1.
-    apply le_n_0_eq in Hso2.
-    subst. reflexivity.
-  -
+
+
+
+(* Theorem replay_state_is_consistent : *)
+(*   forall (* ..for all window size 'ws' and transaction log 'tlog' *)
+(*        containing 'high_wm_offset' entries... *) *)
+(*     (ws : nat) *)
+(*     (tlog : Tlog) *)
+(*     (* ...any two followers starting from a valid offset... *) *)
+(*     start_offset1 (Hso1 : start_offset1 <= length tlog) *)
+(*     start_offset2 (Hso2 : start_offset2 <= length tlog) *)
+(*   , (* ...will eventually reach the same state: *) *)
+(*     replay tlog (initial_state ws start_offset1) = *)
+(*     replay tlog (initial_state ws start_offset2). *)
+(* Proof. *)
+(*   intros. *)
+(*   unfold initial_state. *)
+(*   remember (rev tlog) as tlog'. *)
+(*   induction rtlog; *)
+(*     rewrite <- rev_length in *. *)
+(*   - (* Tlog is empty *) *)
+(*     simpl in *. destruct Heqrtlog. *)
+(*     apply le_n_0_eq in Hso1. *)
+(*     apply le_n_0_eq in Hso2. *)
+(*     subst. reflexivity. *)
+(*   - *)
