src/ToySep.v
@@ -1,0 +1,183 @@
+(** This module contains toy implementation of separation logic *)
+Require Coq.Vectors.Fin.
+Require Coq.Vectors.Vector.
+Module Fin := Coq.Vectors.Fin.
+Module Vec := Coq.Vectors.Vector.
+
+Module IOHandler.
+  Variable N_actors : nat.
+
+  Definition AID : Set := Fin.t N_actors.
+
+  Inductive HandlerRet {req_t state_t : Type} (req : req_t) {rep_t : req_t -> Set} : Type :=
+  | r_return : forall (reply : rep_t req)
+                 (state : state_t)
+               , HandlerRet req
+  | r_stall : HandlerRet req.
+
+  Record t : Type :=
+    {
+      h_state : Set;
+      h_req : Set;
+      h_ret : h_req -> Set;
+      (* Nondeterministic: *)
+      h_initial_state : h_state -> Prop;
+      (* Nondeterministic: *)
+      h_eval : forall (state : h_state)
+                 (aid : AID)
+                 (req : h_req)
+                 (ret : @HandlerRet h_req h_state req h_ret)
+               , Prop;
+    }.
+
+  Section Composition.
+    Definition compose_state h1 h2 : Set :=
+      h_state h1 * h_state h2.
+
+    Definition compose_req h1 h2 : Set :=
+      h_req h1 + h_req h2.
+
+    Hint Transparent compose_state.
+
+    Definition compose_ret_t h1 h2 req :=
+      match req with
+      | inl l => h1.(h_ret) l
+      | inr r => h2.(h_ret) r
+      end.
+
+    Hint Transparent compose_ret_t.
+
+    Definition compose_initial_state h1 h2 state :=
+      h1.(h_initial_state) (fst state) /\ h2.(h_initial_state) (snd state).
+
+    Hint Transparent compose_initial_state.
+
+    Definition ComposeHandlerRet h1 h2 req := @HandlerRet (compose_req h1 h2)
+                                                          (compose_state h1 h2)
+                                                          req
+                                                          (compose_ret_t h1 h2).
+
+    Hint Transparent ComposeHandlerRet.
+
+    Definition compose_eval h1 h2
+               (state : compose_state h1 h2)
+               (aid : AID)
+               req
+               (ret : ComposeHandlerRet h1 h2 req) : Prop.
+    Admitted.
+      (* let (s1, s2) := state in *)
+      (* match req with *)
+      (* | inl req => h1.(h_eval) s1 aid req ret *)
+      (* | inr req => h2.(h_eval) s2 aid req ret *)
+      (* end. *)
+
+    Definition compose (h1 h2 : t) :=
+      {| h_state := compose_state h1 h2;
+         h_req   := compose_req h1 h2;
+         h_ret   := fun req => compose_ret_t h1 h2 req;
+         h_initial_state := fun state => compose_initial_state h1 h2 state;
+         h_eval  := fun state aid io result => compose_eval h1 h2 state aid io result
+      |}.
+  End Composition.
+
+  Variable H : t.
+
+  CoInductive Actor {T : t} : Type :=
+  | a_waiting : forall (pending_io : T.(h_req))
+                  (continuation : T.(h_ret) pending_io -> Actor)
+                , Actor
+  | a_dead : Actor.
+
+  Definition Actors := Vec.t (@Actor H) N_actors.
+
+  Definition Trace := list H.(h_req).
+
+  Record ModelState (T : t) : Type :=
+    mkState
+      {
+        m_actors : Actors;
+        m_state  : T.(h_state);
+        m_trace  : Trace;
+      }.
+
+  (* Local Definition init_actors : Actors. *)
+  (*   refine (fix go i := *)
+  (*             match i with *)
+  (*             | 0 => Vec.nil *)
+  (*             | Fin.S i' => Vec.cons (start_actor i) (go i') *)
+  (*             end). *)
+
+
+
+  (* Inductive model_step (s : ModelState) : ModelState -> Prop := *)
+  (* | mod_init : forall s0, H.(h_initial_state) s0 -> *)
+  (*                   mkState init_actors s0 []. *)
+
+  Definition exit {T : t} : @Actor T := a_dead.
+End IOHandler.
+
+Module ExampleModelDefn.
+  Import IOHandler.
+  Local Definition state : Set := nat * bool.
+
+  Inductive io :=
+  | get : io
+  | put : nat -> io
+  | lock : io
+  | unlock : io
+  .
+
+  Local Definition ret_t (io : io) : Set :=
+    match io with
+    | get => nat
+    | _ => True
+    end.
+
+  Local Definition eval_f (s0 : state) (aid : AID) (req : io) : @HandlerRet io state req ret_t :=
+    match req, s0 with
+    | get, (x, _)      => r_return _ x s0
+    | put N, (_, l)    => r_return _ I (N, l)
+    | lock, (x, false) => r_return _ I (x, true)
+    | lock, (x, true)  => r_stall  _
+    | unlock, (x, _)   => r_return _ I (x, false)
+    end.
+
+  Inductive example_eval (s0 : state) (aid : AID) (req : io) : @HandlerRet io state req ret_t -> Prop :=
+  | example_eval1 : example_eval s0 aid req (eval_f s0 aid req).
+
+  Inductive example_initial_state : state -> Prop :=
+  | example_initial_state1 : example_initial_state (0, false).
+
+  Local Definition exampleHandler : IOHandler.t :=
+    {|
+      h_state := state;
+      h_req := io;
+      h_ret := ret_t;
+      h_initial_state := example_initial_state;
+      h_eval := example_eval;
+    |}.
+
+  Notation "'do' V '<-' I ; C" := (@a_waiting exampleHandler (I) (fun V => C))
+                                    (at level 100, C at next level, V ident, right associativity).
+
+  (* Just a demonstration that we can define programs that loop
+  indefinitely, as long as they do IO: *)
+  Local CoFixpoint infinite_loop (aid : AID) : @Actor exampleHandler :=
+    @a_waiting exampleHandler (put 1) (fun ret => infinite_loop aid).
+
+  (* Data race example: *)
+  Local Definition counter_race (_ : AID) : @Actor exampleHandler :=
+    do v <- get;
+    do _ <- put (v + 1);
+    exit.  Notation "'do' I; C" := (do _ <- I ; C)
+                            (at level 100, C at next level, right associativity).
+
+  (* Fixed example: *)
+  Local Definition counter_correct (_ : AID) : @Actor exampleHandler :=
+    do _ <- lock;
+    do v <- get;
+    do _ <- put (v + 1);
+    do _ <- unlock;
+    exit.
+
+End ExampleModelDefn.
